Corrections to buffer and work towards pericondition law for parallel composition

tutorial/utp_csp_buffer.thy
@@ -12,11 +12,10 @@ type_synonym act_buffer = "(st_buffer, ch_buffer) action"
   
 abbreviation DoBuff :: act_buffer where
 "DoBuff \<equiv> (inp\<^bold>?v \<^bold>\<rightarrow> buff :=\<^sub>C (&buff ^\<^sub>u \<langle>\<guillemotleft>v\<guillemotright>\<rangle>)
-           \<box> (#\<^sub>u(&buff) >\<^sub>u 0) &\<^sub>u outp\<^bold>!last\<^sub>u(&buff) \<^bold>\<rightarrow> buff :=\<^sub>C tail\<^sub>u(&buff))"
-  
+           \<box> (#\<^sub>u(&buff) >\<^sub>u 0) &\<^sub>u outp\<^bold>!head\<^sub>u(&buff) \<^bold>\<rightarrow> buff :=\<^sub>C tail\<^sub>u(&buff))"
+
 definition Buffer :: act_buffer where
-"Buffer = buff :=\<^sub>C \<langle>\<rangle> ;; (\<mu> X \<bullet> (inp\<^bold>?v \<^bold>\<rightarrow> buff :=\<^sub>C (&buff ^\<^sub>u \<langle>\<guillemotleft>v\<guillemotright>\<rangle>)
-                             \<box> (#\<^sub>u(&buff) >\<^sub>u 0) &\<^sub>u outp\<^bold>!last\<^sub>u(&buff) \<^bold>\<rightarrow> buff :=\<^sub>C tail\<^sub>u(&buff)) ;; CSP(X))"
+"Buffer = buff :=\<^sub>C \<langle>\<rangle> ;; (\<mu> X \<bullet> DoBuff ;; CSP(X))"
   
 declare image_eqI [closure del]
 declare Healthy_set_image_member [closure del]
@@ -27,13 +26,14 @@ lemma preR_DoBuff: "pre\<^sub>R(DoBuff) = true"
   by (simp add: rdes closure wp unrest usubst alpha)
     
 lemma periR_DoBuff: 
-  "peri\<^sub>R(DoBuff) = (((\<Squnion> v \<bullet> (inp\<cdot>\<guillemotleft>v\<guillemotright>)\<^sub>u \<notin>\<^sub>u $ref\<acute>) \<and> $tr\<acute> =\<^sub>u $tr) \<and>
-                     ($tr\<acute> =\<^sub>u $tr \<and> \<lceil>(outp\<cdot>last\<^sub>u(&buff))\<^sub>u\<rceil>\<^sub>S\<^sub>< \<notin>\<^sub>u $ref\<acute>) \<triangleleft> #\<^sub>u($st:buff) >\<^sub>u 0 \<triangleright> ($tr\<acute> =\<^sub>u $tr))"
+  "peri\<^sub>R(DoBuff) = 
+     ((\<Squnion> v \<bullet> (inp\<cdot>\<guillemotleft>v\<guillemotright>)\<^sub>u \<notin>\<^sub>u $ref\<acute>) \<and> $tr\<acute> =\<^sub>u $tr \<and>
+      (\<lceil>(outp\<cdot>head\<^sub>u(&buff))\<^sub>u\<rceil>\<^sub>S\<^sub>< \<notin>\<^sub>u $ref\<acute>) \<triangleleft> #\<^sub>u($st:buff) >\<^sub>u 0 \<triangleright> true)"
   by (simp add: rdes closure wp unrest usubst alpha, rel_auto)
-
+  
 lemma postR_DoBuff: 
   "post\<^sub>R(DoBuff) = ((\<Sqinter> v \<bullet> $tr\<acute> =\<^sub>u $tr ^\<^sub>u \<langle>(inp\<cdot>\<guillemotleft>v\<guillemotright>)\<^sub>u\<rangle> \<and> \<lceil>buff := &buff ^\<^sub>u \<langle>\<guillemotleft>v\<guillemotright>\<rangle>\<rceil>\<^sub>S) \<or>
-                    #\<^sub>u($st:buff) >\<^sub>u 0 \<and> $tr\<acute> =\<^sub>u $tr ^\<^sub>u \<langle>\<lceil>(outp\<cdot>last\<^sub>u(&buff))\<^sub>u\<rceil>\<^sub>S\<^sub><\<rangle> \<and> \<lceil>buff := tail\<^sub>u(&buff)\<rceil>\<^sub>S)"
+                    #\<^sub>u($st:buff) >\<^sub>u 0 \<and> $tr\<acute> =\<^sub>u $tr ^\<^sub>u \<langle>\<lceil>(outp\<cdot>head\<^sub>u(&buff))\<^sub>u\<rceil>\<^sub>S\<^sub><\<rangle> \<and> \<lceil>buff := tail\<^sub>u(&buff)\<rceil>\<^sub>S)"
   by (simp add: rdes closure wp unrest usubst alpha)
   
 lemma preR_Buffer: "pre\<^sub>R(Buffer) = true"
